helper mono, spsStep mono iff uspecWell

untimed/SpsStep.thy
@@ -7,58 +7,65 @@ begin
 default_sort type
 type_synonym 'm SPS = "'m SPF uspec"
 
-definition spsStep_h_test::"((channel\<rightharpoonup>'m::message) \<Rightarrow> 'm SPS) \<Rightarrow> ((channel\<rightharpoonup>'m::message) \<Rightarrow> 'm SPF) set"where
-"spsStep_h_test= (\<lambda> h. {(\<lambda>e. spf) |spf e. spf \<in> (Rep_rev_uspec (h e))})"
+definition spsStep_h::"((channel\<rightharpoonup>'m::message) \<Rightarrow> 'm SPS)\<rightarrow> ((channel\<rightharpoonup>'m::message) \<Rightarrow> 'm SPF) set rev"where
+"spsStep_h= (\<Lambda> h. (Rev {(\<lambda>e. if e = x then spf else ufLeast (ufDom\<cdot> spf) (ufDom\<cdot> spf)) | spf x. spf \<in> (Rep_rev_uspec (h x))}))"
 
-definition spsStep_h::"((channel\<rightharpoonup>'m::message) \<Rightarrow> 'm SPS)\<rightarrow> ((channel\<rightharpoonup>'m::message) \<Rightarrow> 'm SPF) set"where
-"spsStep_h= (\<Lambda> h. {(\<lambda>e. spf) |spf e. spf \<in> (Rep_rev_uspec (h e))})"
-
-lemma spsStep_h_mono[simp]:"monofun (\<lambda>h::(channel \<Rightarrow> 'a::message option) \<Rightarrow> ('a stream\<^sup>\<Omega>) ufun uspec. {\<lambda>e::channel \<Rightarrow> 'a option. spf |spf::('a stream\<^sup>\<Omega>) ufun. \<exists>e::channel \<Rightarrow> 'a option. spf \<in> Rep_rev_uspec (h e)})"
+lemma spsStep_h_mono[simp]:"monofun (\<lambda> h. Rev {(\<lambda>e::(channel\<rightharpoonup>'m::message). if e = z then spf else ufLeast (ufDom\<cdot> spf) (ufDom\<cdot> spf)) |(spf::'m SPF) z. spf \<in> (Rep_rev_uspec (h z))})"
 proof(rule monofunI)
-  fix x y::"(channel \<Rightarrow> 'a option) \<Rightarrow> ('a stream\<^sup>\<Omega>) ufun uspec"
+  fix x y::"(channel \<Rightarrow> 'm option) \<Rightarrow> 'm SPS"
   assume a1:"x \<sqsubseteq> y"
-  show "{\<lambda>e::channel \<Rightarrow> 'a option. spf |spf::('a stream\<^sup>\<Omega>) ufun. \<exists>e::channel \<Rightarrow> 'a option. spf \<in> Rep_rev_uspec (x e)} \<sqsubseteq>
-       {\<lambda>e::channel \<Rightarrow> 'a option. spf |spf::('a stream\<^sup>\<Omega>) ufun. \<exists>e::channel \<Rightarrow> 'a option. spf \<in> Rep_rev_uspec (y e)}"
-    sorry
+  have "\<And>z. Rep_rev_uspec (y z) \<subseteq> Rep_rev_uspec (x z)"
+    by (metis less_set_def rep_uspec_belowI a1 fun_belowD inv_rev_rep_upsec_below)
+  then have "\<And>z spf. spf \<in> Rep_rev_uspec (y z) \<Longrightarrow> spf \<in> Rep_rev_uspec (x z)"
+    by blast
+  then have "{\<lambda>e. if e = z then spf else ufLeast (ufDom\<cdot>spf) (ufDom\<cdot>spf) |spf z. spf \<in> Rep_rev_uspec (y z)} \<subseteq>
+             {\<lambda>e. if e = z then spf else ufLeast (ufDom\<cdot>spf) (ufDom\<cdot>spf) |spf z. spf \<in> Rep_rev_uspec (x z)}"
+    by blast
+  then show "Rev {\<lambda>e. if e = z then spf else ufLeast (ufDom\<cdot>spf) (ufDom\<cdot>spf) |spf z. spf \<in> Rep_rev_uspec (x z)} \<sqsubseteq>
+       Rev {\<lambda>e. if e = z then spf else ufLeast (ufDom\<cdot>spf) (ufDom\<cdot>spf) |spf z. spf \<in> Rep_rev_uspec (y z)}"
+    by(simp add: less_set_def)
 qed
   
-    
-    
-lemma spsStep_h_test_cont[simp]:"cont(spsStep_h_test)"
-proof(simp add: spsStep_h_test_def, rule Cont.contI2, simp)
-  fix Y::"nat \<Rightarrow> (channel \<Rightarrow> 'a option) \<Rightarrow> ('a stream\<^sup>\<Omega>) ufun uspec"
-  assume a1:"chain Y"
-  assume a2:"chain (\<lambda>i::nat. {\<lambda>e::channel \<Rightarrow> 'a option. spf |spf::('a stream\<^sup>\<Omega>) ufun. \<exists>e::channel \<Rightarrow> 'a option. spf \<in> Rep_rev_uspec (Y i e)})"
-  show "{\<lambda>e::channel \<Rightarrow> 'a option. spf |spf::('a stream\<^sup>\<Omega>) ufun. \<exists>e::channel \<Rightarrow> 'a option. spf \<in> Rep_rev_uspec ((\<Squnion>i::nat. Y i) e)} \<sqsubseteq>
-       (\<Squnion>i::nat. {\<lambda>e::channel \<Rightarrow> 'a option. spf |spf::('a stream\<^sup>\<Omega>) ufun. \<exists>e::channel \<Rightarrow> 'a option. spf \<in> Rep_rev_uspec (Y i e)})"
-    sorry
-qed
-  
-lemma spsStep_h_cont[simp]:"cont (\<lambda> (h::((channel \<Rightarrow> 'm::message option) \<Rightarrow> ('m stream\<^sup>\<Omega>) ufun uspec)). {(\<lambda>e::(channel\<rightharpoonup>'m::message). spf) |(spf::('m stream\<^sup>\<Omega>) ufun) (e::channel \<Rightarrow> 'm option). spf \<in> (Rep_rev_uspec (h e))})"
-  by(insert spsStep_h_test_cont, simp add:spsStep_h_test_def)
-
-lemma spsStep_h_insert:"spsStep_h\<cdot> f = {(\<lambda>e. spf) |spf e. spf \<in> (Rep_rev_uspec (f e))}"
-  apply (simp add: spsStep_h_def, subst beta_cfun, auto)
-  by(insert spsStep_h_cont, simp)
-
-(* like spfStep, copy & pasteonly on SPS *)
-fun spsStep :: "channel set discr \<Rightarrow> channel set discr \<Rightarrow> ((channel\<rightharpoonup>'m::message) \<Rightarrow> 'm SPS) \<rightarrow> 'm SPS" where
-"spsStep (Discr In) (Discr Out) = (\<Lambda> h. Abs_rev_uspec {spfStep In Out\<cdot>g | g. g \<in>(spsStep_h\<cdot>h)})"
-
-lemma spsStep_mono[simp]:"monofun (\<lambda>h::(channel \<Rightarrow> 'a::message option) \<Rightarrow> ('a stream\<^sup>\<Omega>) ufun uspec. Abs_rev_uspec {spfStep In Out\<cdot>g |g::(channel \<Rightarrow> 'a option) \<Rightarrow> ('a stream\<^sup>\<Omega>) ufun. g \<in> spsStep_h\<cdot>h})"
+      
+lemma spsStep_h_cont[simp]:"cont (\<lambda> h. (Rev {(\<lambda>e::(channel\<rightharpoonup>'m::message). if e = x then spf else ufLeast (ufDom\<cdot> spf) (ufDom\<cdot> spf)) | (spf::'m SPF) x. spf \<in> (Rep_rev_uspec (h x))}))"
   sorry
 
-lemma spsStep_h_elem:"f \<in> (\<Squnion>i::nat. spsStep_h\<cdot>(Y i)) \<Longrightarrow> f \<in> (spsStep_h\<cdot>(Y i))"
-  sorry    
+lemma spsStep_h_insert:"spsStep_h\<cdot> f = (Rev {(\<lambda>e. if e = x then spf else ufLeast (ufDom\<cdot> spf) (ufDom\<cdot> spf)) | spf x. spf \<in> (Rep_rev_uspec (f x))})"
+  by(simp add: spsStep_h_def)
+    
+(* like spfStep, copy & pasteonly on SPS *)
+fun spsStep :: "channel set discr \<Rightarrow> channel set discr \<Rightarrow> ((channel\<rightharpoonup>'m::message) \<Rightarrow> 'm SPS) \<rightarrow> 'm SPS" where
+"spsStep (Discr In) (Discr Out) = (\<Lambda> h. Abs_rev_uspec {spfStep In Out\<cdot>g | g. g \<in> inv Rev (spsStep_h\<cdot>h)})"
 
-lemma spsStep_cont[simp]:"cont (\<lambda>h. Abs_rev_uspec {spfStep In Out\<cdot>g | g. g \<in>(spsStep_h\<cdot>h)})"
+lemma spsStep_mono[simp]:"monofun (\<lambda>h::(channel \<Rightarrow> 'a::message option) \<Rightarrow> ('a stream\<^sup>\<Omega>) ufun uspec. Abs_rev_uspec {spfStep In Out\<cdot>g |g::(channel \<Rightarrow> 'a option) \<Rightarrow> ('a stream\<^sup>\<Omega>) ufun. g \<in> inv Rev (spsStep_h\<cdot>h)})"
+proof(rule monofunI)
+  fix x y::"(channel \<Rightarrow> 'm::message option) \<Rightarrow> 'm SPS" 
+  assume a1: "x \<sqsubseteq> y"
+  have "(spsStep_h\<cdot>x) \<sqsubseteq> (spsStep_h\<cdot>y)" 
+    by (simp add: a1 monofun_cfun_arg)
+  then have "inv Rev(spsStep_h\<cdot>y) \<subseteq> inv Rev (spsStep_h\<cdot>x)"
+    by (metis (full_types) SetPcpo.less_set_def below_rev.elims(2) inv_rev_rev)
+  then have "\<And>g. g \<in> inv Rev(spsStep_h\<cdot>y) \<Longrightarrow> g \<in> inv Rev (spsStep_h\<cdot>x)"
+    by blast
+  then have h1:"{spfStep In Out\<cdot>g |g. g \<in> inv Rev (spsStep_h\<cdot>y)} \<sqsubseteq>{spfStep In Out\<cdot>g |g. g \<in> inv Rev (spsStep_h\<cdot>x)}"
+    by (smt Collect_mono SetPcpo.less_set_def)
+  have h2:"uspecWell {spfStep In Out\<cdot>g |g::(channel \<Rightarrow> 'm option) \<Rightarrow> ('m stream\<^sup>\<Omega>) ufun. g \<in> inv Rev (spsStep_h\<cdot>x)}"
+    sorry
+  have h3:"uspecWell {spfStep In Out\<cdot>g |g::(channel \<Rightarrow> 'm option) \<Rightarrow> ('m stream\<^sup>\<Omega>) ufun. g \<in> inv Rev (spsStep_h\<cdot>y)}"
+    sorry
+  show "Abs_rev_uspec {spfStep In Out\<cdot>g |g. g \<in> inv Rev (spsStep_h\<cdot>x)} \<sqsubseteq>
+       Abs_rev_uspec {spfStep In Out\<cdot>g |g. g \<in> inv Rev (spsStep_h\<cdot>y)}"
+    by (metis (mono_tags, lifting) h1 h2 h3 rep_abs_rev_simp uspec_belowI)
+qed
+  
+lemma spsStep_cont[simp]:"cont (\<lambda>h. Abs_rev_uspec {spfStep In Out\<cdot>g | g. g \<in>inv Rev (spsStep_h\<cdot>h)})"
 proof(rule Cont.contI2, simp)
-  fix Y::"nat \<Rightarrow> (channel \<Rightarrow> 'a option) \<Rightarrow> ('a stream\<^sup>\<Omega>) ufun uspec"
+  fix Y::"nat \<Rightarrow> ((channel \<Rightarrow> 'm::message option) \<Rightarrow> 'm SPS)"
   assume a1:"chain Y"
-  assume a2:"chain (\<lambda>i::nat. Abs_rev_uspec {spfStep In Out\<cdot>g |g::(channel \<Rightarrow> 'a option) \<Rightarrow> ('a stream\<^sup>\<Omega>) ufun. g \<in> spsStep_h\<cdot>(Y i)})"
-  show "Abs_rev_uspec {spfStep In Out\<cdot>g |g::(channel \<Rightarrow> 'a option) \<Rightarrow> ('a stream\<^sup>\<Omega>) ufun. g \<in> spsStep_h\<cdot>(\<Squnion>i::nat. Y i)} \<sqsubseteq>
-       (\<Squnion>i::nat. Abs_rev_uspec {spfStep In Out\<cdot>g |g::(channel \<Rightarrow> 'a option) \<Rightarrow> ('a stream\<^sup>\<Omega>) ufun. g \<in> spsStep_h\<cdot>(Y i)})"
-  apply(simp add: a1 contlub_cfun_fun contlub_cfun_arg spsStep_h_elem)
+  assume a2:"chain (\<lambda>i::nat. Abs_rev_uspec {spfStep In Out\<cdot>g |g. g \<in> inv Rev (spsStep_h\<cdot>(Y i))})"
+  show "Abs_rev_uspec {spfStep In Out\<cdot>g |g. g \<in> inv Rev (spsStep_h\<cdot>(\<Squnion>i::nat. Y i))} \<sqsubseteq>
+       (\<Squnion>i::nat. Abs_rev_uspec {spfStep In Out\<cdot>g |g. g \<in> inv Rev (spsStep_h\<cdot>(Y i))})"
+  apply(simp add: a1 contlub_cfun_fun contlub_cfun_arg)
     sorry
 qed
   
